synthesize motive for first header

Examples.lean
@@ -4,14 +4,14 @@ mutual
 
 iit Con : Type where
 | nil : Con
-| ext : (Γ : Con) → (A : Ty Γ) → Con
+--| ext : (Γ : Con) → (A : Ty Γ) → Con
 
 iit Ty : (Γ : Con) → Type where
 | U : (Δ : Con) → Ty Δ
-| pi : ∀ (Γ : Con) (A : Ty Γ) (B : Ty (Con.ext Γ A)), Ty Γ
+--| pi : ∀ (Γ : Con) (A : Ty Γ) (B : Ty (Con.ext Γ A)), Ty Γ
 
-iit Tm : (Γ : Con) → (A : Ty Γ) → Type where
-| El : (Γ : Con) → Tm Γ (Ty.U Γ)
+--iit Tm : (Γ : Con) → (A : Ty Γ) → Type where
+--| El : (Γ : Con) → Tm Γ (Ty.U Γ)
 
 --iit Subb : (Δ Γ : Con) → Type where
 --| swap : (Δ Γ : Con) → (A : Subb Γ Δ) → Subb Δ Γ
@@ -29,93 +29,211 @@ end
 
 open IIT
 
-noncomputable def Cont_total : Con.tot := by
+--set_option pp.all true
+
+noncomputable def Con_total : Con.tot := by
+  totalityOuter 0 [Con, Ty] [Con.nil] [Ty.U]
+  refine @Con.E.rec
+          (fun Γ.e => ∀ Γ.w, PSigma (Con.r Con.m Ty.m Con.nil.m Ty.U.m { fst := Γ.e, snd := Γ.w }))
+          (fun A.e => ∀ Γ Γ.m (Γ.r : Con.r Con.m Ty.m Con.nil.m Ty.U.m Γ Γ.m) A.w, 
+            PSigma (@Ty.r Con.m Ty.m Con.nil.m Ty.U.m Γ Γ.m { fst := A.e, snd := A.w })) ?_ ?_ S.E S.w
+  skip --TODO finde heraus, wie refine die typen der loecher inferiert
+
+#check @Con.E.rec
+
+#exit
+noncomputable def Con_total : Con.tot := by
   totalityOuter 0 [Con, Ty, Tm] [Con.nil, Con.ext] [Ty.U, Ty.pi] [Tm.El]
-  cases sMain with
-  | PSigma.mk Γ.e Γ.w =>
-    apply @Con.E.rec
-            (fun Γ.e => ∀ Γ.w, PSigma (Con.r Con.m Ty.m Tm.m Con.nil.m Con.ext.m Ty.U.m Ty.pi.m Tm.El.m { fst := Γ.e, snd := Γ.w }))
-            (fun A.e => ∀ Γ Γ.m (Γ.r : Con.r Con.m Ty.m Tm.m Con.nil.m Con.ext.m Ty.U.m Ty.pi.m Tm.El.m Γ Γ.m) A.w, 
-              PSigma (@Ty.r Con.m Ty.m Tm.m Con.nil.m Con.ext.m Ty.U.m Ty.pi.m Tm.El.m Γ Γ.m { fst := A.e, snd := A.w }))
-            (fun t.e => PUnit)
-    focus
-      intro Γ.w'
-      apply PSigma.mk
-      apply Con.nil.r
-    focus
-      intros _ _ ih1 ih2 Γ.w'
-      apply PSigma.mk
-      apply Con.ext.r (Γ.r := (ih1 _).snd) (A.r := (ih2 _ _ _ _).snd)
-      repeat { cases Γ.w'; assumption }
-      apply (ih1 _).snd
-    focus
-      intros Δ _ Γ' _ _ U.w
-      have e : Γ'.1 = Δ := by { cases U.w; rfl }
-      induction e
-      apply PSigma.mk
-      apply Ty.U.r
-      assumption
-    focus
-      intros Γ A B Γ.r A.r B.r Γ' Γ'.m Γ'.r π.w
-      have e : Γ'.1 = Γ := by { cases π.w; rfl }
-      induction e
-      apply PSigma.mk
-      apply Ty.pi.r (Γ.r := Γ'.r) (A.r := (A.r _ _ _ _).snd) (B.r := (B.r _ _ _ _).snd)
-      cases π.w
-      assumption
-      assumption
-      cases π.w
-      assumption
-      apply Con.ext.r
-      assumption
-      cases π.w
-      apply (A.r _ _ _ _).snd
-    focus
-      intros
-      exact ()
+  apply @Con.E.rec
+          (fun Γ.e => ∀ Γ.w, PSigma (Con.r Con.m Ty.m Tm.m Con.nil.m Con.ext.m Ty.U.m Ty.pi.m Tm.El.m { fst := Γ.e, snd := Γ.w }))
+          (fun A.e => ∀ Γ Γ.m (Γ.r : Con.r Con.m Ty.m Tm.m Con.nil.m Con.ext.m Ty.U.m Ty.pi.m Tm.El.m Γ Γ.m) A.w, 
+            PSigma (@Ty.r Con.m Ty.m Tm.m Con.nil.m Con.ext.m Ty.U.m Ty.pi.m Tm.El.m Γ Γ.m { fst := A.e, snd := A.w }))
+          (fun t.e => PUnit)
+  focus
+    intro Γ.w'
+    apply PSigma.mk
+    apply Con.nil.r
+  focus
+    intros _ _ ih1 ih2 Γ.w'
+    apply PSigma.mk
+    apply Con.ext.r (Γ.r := (ih1 _).snd) (A.r := (ih2 _ _ _ _).snd)
+    repeat { cases Γ.w'; assumption }
+    apply (ih1 _).snd
+  focus
+    intros Δ _ Γ' _ _ U.w
+    have e : Γ'.1 = Δ := by { cases U.w; rfl }
+    induction e
+    apply PSigma.mk
+    apply Ty.U.r
+    assumption
+  focus
+    intros Γ A B Γ.r A.r B.r Γ' Γ'.m Γ'.r π.w
+    have e : Γ'.1 = Γ := by { cases π.w; rfl }
+    induction e
+    apply PSigma.mk
+    apply Ty.pi.r (Γ.r := Γ'.r) (A.r := (A.r _ _ _ _).snd) (B.r := (B.r _ _ _ _).snd)
+    cases π.w
+    assumption
+    assumption
+    cases π.w
+    assumption
+    apply Con.ext.r
+    assumption
+    cases π.w
+    apply (A.r _ _ _ _).snd
+  focus
+    intros
+    exact ()
 
 noncomputable def Ty_total : Ty.tot := by
   totalityOuter 1 [Con, Ty, Tm] [Con.nil, Con.ext] [Ty.U, Ty.pi] [Tm.El]
-  cases sMain with
-  | PSigma.mk A.e A.w =>
-    apply @Ty.E.rec
-            (fun Γ.e => ∀ Γ.w, PSigma (Con.r Con.m Ty.m Tm.m Con.nil.m Con.ext.m Ty.U.m Ty.pi.m Tm.El.m { fst := Γ.e, snd := Γ.w }))
-            (fun A.e => ∀ Γ Γ.m (Γ.r : Con.r Con.m Ty.m Tm.m Con.nil.m Con.ext.m Ty.U.m Ty.pi.m Tm.El.m Γ Γ.m) A.w, 
-              PSigma (@Ty.r Con.m Ty.m Tm.m Con.nil.m Con.ext.m Ty.U.m Ty.pi.m Tm.El.m Γ Γ.m { fst := A.e, snd := A.w }))
-            (fun t.e => PUnit)
-    focus
-      intro Γ.w'
-      apply PSigma.mk
-      apply Con.nil.r
-    focus
-      intros _ _ ih1 ih2 Γ.w'
-      apply PSigma.mk
-      apply Con.ext.r (Γ.r := (ih1 _).snd) (A.r := (ih2 _ _ _ _).snd)
-      repeat { cases Γ.w'; assumption }
-      apply (ih1 _).snd
-    focus
-      intros Δ _ Γ' _ _ U.w
-      have e : Γ'.1 = Δ := by { cases U.w; rfl }
-      induction e
-      apply PSigma.mk
-      apply Ty.U.r
-      assumption
-    focus
-      intros Γ A B Γ.r A.r B.r Γ' Γ'.m Γ'.r π.w
-      have e : Γ'.1 = Γ := by { cases π.w; rfl }
-      induction e
-      apply PSigma.mk
-      apply Ty.pi.r (Γ.r := Γ'.r) (A.r := (A.r _ _ _ _).snd) (B.r := (B.r _ _ _ _).snd)
-      cases π.w
-      assumption
-      assumption
-      cases π.w
-      assumption
-      apply Con.ext.r
-      assumption
-      cases π.w
-      apply (A.r _ _ _ _).snd
-    focus
-      intros
-      exact ()
+  apply @Ty.E.rec
+          (fun Γ.e => ∀ Γ.w, PSigma (Con.r Con.m Ty.m Tm.m Con.nil.m Con.ext.m Ty.U.m Ty.pi.m Tm.El.m { fst := Γ.e, snd := Γ.w }))
+          (fun A.e => ∀ Γ Γ.m (Γ.r : Con.r Con.m Ty.m Tm.m Con.nil.m Con.ext.m Ty.U.m Ty.pi.m Tm.El.m Γ Γ.m) A.w, 
+            PSigma (@Ty.r Con.m Ty.m Tm.m Con.nil.m Con.ext.m Ty.U.m Ty.pi.m Tm.El.m Γ Γ.m { fst := A.e, snd := A.w }))
+          (fun t.e => PUnit)
+  focus
+    intro Γ.w'
+    apply PSigma.mk
+    apply Con.nil.r
+  focus
+    intros _ _ ih1 ih2 Γ.w'
+    apply PSigma.mk
+    apply Con.ext.r (Γ.r := (ih1 _).snd) (A.r := (ih2 _ _ _ _).snd)
+    repeat { cases Γ.w'; assumption }
+    apply (ih1 _).snd
+  focus
+    intros Δ _ Γ' _ _ U.w
+    have e : Γ'.1 = Δ := by { cases U.w; rfl }
+    induction e
+    apply PSigma.mk
+    apply Ty.U.r
     assumption
+  focus
+    intros Γ A B Γ.r A.r B.r Γ' Γ'.m Γ'.r π.w
+    have e : Γ'.1 = Γ := by { cases π.w; rfl }
+    induction e
+    apply PSigma.mk
+    apply Ty.pi.r (Γ.r := Γ'.r) (A.r := (A.r _ _ _ _).snd) (B.r := (B.r _ _ _ _).snd)
+    cases π.w
+    assumption
+    assumption
+    cases π.w 
+    assumption
+    apply Con.ext.r
+    assumption
+    cases π.w
+    apply (A.r _ _ _ _).snd
+  focus
+    intros
+    exact ()
+  assumption
+
+#check Tm.El.r
+
+noncomputable def Tm_total : Tm.tot := by
+  totalityOuter 2 [Con, Ty, Tm] [Con.nil, Con.ext] [Ty.U, Ty.pi] [Tm.El]
+/-  apply @Tm.E.rec
+          (fun Γ.e => ∀ Γ.w, PSigma (Con.r Con.m Ty.m Tm.m Con.nil.m Con.ext.m Ty.U.m Ty.pi.m Tm.El.m { fst := Γ.e, snd := Γ.w }))
+          (fun A.e => ∀ Γ Γ.m (Γ.r : Con.r Con.m Ty.m Tm.m Con.nil.m Con.ext.m Ty.U.m Ty.pi.m Tm.El.m Γ Γ.m) A.w, 
+            PSigma (@Ty.r Con.m Ty.m Tm.m Con.nil.m Con.ext.m Ty.U.m Ty.pi.m Tm.El.m Γ Γ.m { fst := A.e, snd := A.w }))
+          (fun t.e => ∀ Γ Γ.m (Γ.r : Con.r Con.m Ty.m Tm.m Con.nil.m Con.ext.m Ty.U.m Ty.pi.m Tm.El.m Γ Γ.m)
+                        A A.m (A.r : @Ty.r Con.m Ty.m Tm.m Con.nil.m Con.ext.m Ty.U.m Ty.pi.m Tm.El.m Γ Γ.m A A.m) t.w,
+            PSigma (@Tm.r Con.m Ty.m Tm.m Con.nil.m Con.ext.m Ty.U.m Ty.pi.m Tm.El.m Γ Γ.m A A.m { fst := t.e, snd := t.w}))
+  focus
+    intro Γ.w'
+    apply PSigma.mk
+    apply Con.nil.r
+  focus
+    intros _ _ ih1 ih2 Γ.w'
+    apply PSigma.mk
+    apply Con.ext.r (Γ.r := (ih1 _).snd) (A.r := (ih2 _ _ _ _).snd)
+    repeat { cases Γ.w'; assumption }
+    apply (ih1 _).snd
+  focus
+    intros Δ _ Γ' _ _ U.w
+    have e : Γ'.1 = Δ := by { cases U.w; rfl }
+    induction e
+    apply PSigma.mk
+    apply Ty.U.r
+    assumption
+  focus
+    intros Γ A B Γ.r A.r B.r Γ' Γ'.m Γ'.r π.w
+    have e : Γ'.1 = Γ := by { cases π.w; rfl }
+    induction e
+    apply PSigma.mk
+    apply Ty.pi.r (Γ.r := Γ'.r) (A.r := (A.r _ _ _ _).snd) (B.r := (B.r _ _ _ _).snd)
+    cases π.w
+    assumption
+    assumption
+    cases π.w
+    assumption
+    apply Con.ext.r
+    assumption
+    cases π.w
+    apply (A.r _ _ _ _).snd
+  focus
+    intros Γ.E Γ.r Γ' Γ'.m Γ'.r A A.m A.r El.w
+    have e : (Γ'.1 = Γ.E) ∧ (A.1 = Ty.U.E Γ'.1) := by {
+      cases Γ';
+      cases A;
+      cases El.w;
+      apply And.intro;
+      rfl;
+      rfl }
+    cases Γ' with
+    | mk Γ'.e Γ'.w =>
+      cases A
+      cases e.1
+      cases e.2
+      clear e
+      refine PSigma.mk ?_ ?_
+      --have e : A.m = Ty.U.m Γ'.m := by { cases A.r; rfl }
+      --induction e
+      --skip-/
+
+#check Tm.Eld.r
+
+
+inductive fivefive : (n : Nat) → Fin n → Prop where
+| mk : fivefive 10 5
+
+example (m x) (q : 5 < m) (p : fivefive m x) : (x = { val := 5, isLt := q }) := by
+  cases p
+  rfl
+
+mutual
+
+inductive ConE : Type where
+|  nilE : ConE
+|  extE : ConE → TyE → ConE
+
+inductive TyE : Type where
+|  UE : ConE → TyE
+|  piE : ConE → TyE → TyE → TyE
+
+inductive TmE : Type where
+|  ElE : ConE → TmE
+
+end
+
+mutual
+
+inductive Conw : ConE → Prop where
+| nilw : Conw ConE.nilE
+| extw : (ΓE : ConE) → Conw ΓE → (AE : TyE) → Tyw ΓE AE → Conw (ConE.extE ΓE AE)
+
+inductive Tyw : ConE → TyE → Prop where
+| Uw : (ΓE : ConE) → Conw ΓE → Tyw ΓE (TyE.UE ΓE)
+| piw : (ΓE : ConE) → Conw ΓE → (AE : TyE) → Tyw ΓE AE → (BE : TyE) → Tyw (ConE.extE ΓE AE) BE → Tyw ΓE (TyE.piE ΓE AE BE)
+
+inductive Tmw : ConE → TyE → TmE → Prop where
+| Elw : (ΓE : ConE) → Conw ΓE → Tmw ΓE (TyE.UE ΓE) (TmE.ElE ΓE)
+
+end
+
+example (ΓE ΓE' AE) (w : Tmw ΓE AE (TmE.ElE ΓE')) : (ΓE = ΓE') ∧ (AE = TyE.UE ΓE) := by
+  cases w
+  apply And.intro
+  rfl
+  rfl
